wip

libcrux-ml-dsa/proofs/fstar/extraction/Libcrux_ml_dsa.Simd.Avx2.Arithmetic.fst
@@ -91,6 +91,8 @@ let montgomery_multiply_by_constant
 unfold let montgomery_multiply_spec__i32_extended64_mul (x y: i32) : i64 =
   (cast (x <: i32) <: i64) *! (cast (y <: i32) <: i64)
 
+
+[@@ "opaque_to_smt"]
 let montgomery_multiply_spec (x y: i32) : i32 =
   let x_mul_y:i64 = montgomery_multiply_spec__i32_extended64_mul x y in
   let lhs:i32 = cast (x_mul_y >>! mk_i32 32 <: i64) <: i32 in
@@ -141,7 +143,7 @@ let montgomery_multiply_spec_rw (x y: i32) : Lemma ((let x_mul_y:i64 = montgomer
     i32
   in
   Core.Num.impl_i32__wrapping_sub lhs rhs) == montgomery_multiply_spec x y)
-  = ()
+  = admit ()
 
 [@@FStar.Tactics.postprocess_with ( fun _ -> 
   let open Tactics.Circuits in
@@ -221,31 +223,45 @@ let montgomery_multiply (lhs rhs: Core_models.Abstractions.Bitvec.t_BitVec (mk_u
 module BV_LEMMAS = Core_models.Abstractions.Bitvec.Int_vec_interp
 
 
+// BV_LEMMAS.e_ee_1__impl__to_i32x8 (BV_LEMMAS.e_ee_1__impl__from_i32x8
+
+
+// ///Lemma that asserts that applying BitVec :: < 256 > :: from and then i32x8 :: from is the identity.
+// let e_ee_1__lemma_cancel_iv'
+//   (x: Core_models.Abstractions.Funarr.t_FunArray (mk_u64 8) i32) 
+//   (i: u64 {v i < 8})
+//   : Lemma
+//       (ensures (BV_LEMMAS.e_ee_1__impl__to_i32x8 (BV_LEMMAS.e_ee_1__impl__from_i32x8 x)) i == x i)
+//       [
+//         SMTPat
+//         (BV_LEMMAS.e_ee_1__impl__to_i32x8 (BV_LEMMAS.e_ee_1__impl__from_i32x8 x) i)
+//       ]
+//       = admit ()
+
 ///Lemma that asserts that applying BitVec :: < 256 > :: from and then i32x8 :: from is the identity.
-let e_ee_1__lemma_cancel_iv'
+let e_ee_1__lemma_cancel_iv'2
   (x: Core_models.Abstractions.Funarr.t_FunArray (mk_u64 8) i32) 
-  (i: u64 {v i < 8})
   : Lemma
-      (ensures
-        (BV_LEMMAS.e_ee_1__impl__to_i32x8 (BV_LEMMAS.e_ee_1__impl__from_i32x8 x
-              <:
-              Core_models.Abstractions.Bitvec.t_BitVec (mk_u64 256))
-          <:
-          Core_models.Abstractions.Funarr.t_FunArray (mk_u64 8) i32) i ==
-        x i)
+      (ensures (BV_LEMMAS.e_ee_1__impl__to_i32x8 (BV_LEMMAS.e_ee_1__impl__from_i32x8 x)) == x)
       [
         SMTPat
-        (BV_LEMMAS.e_ee_1__impl__to_i32x8 (BV_LEMMAS.e_ee_1__impl__from_i32x8 x) i)
+        (BV_LEMMAS.e_ee_1__impl__to_i32x8 (BV_LEMMAS.e_ee_1__impl__from_i32x8 x))
       ]
       = admit ()
 
 
-let hey lhs rhs: squash (
+#set-options "--fuel 2 --ifuel 2 --z3rlimit 300"
+let montgomery_multiply_lemma lhs rhs: Lemma (
         Core_models.Abstractions.Bitvec.Int_vec_interp.e_ee_1__impl__to_i32x8 (montgomery_multiply lhs rhs) (mk_u64 0)
      == montgomery_multiply_spec 
           (Core_models.Abstractions.Bitvec.Int_vec_interp.e_ee_1__impl__to_i32x8 lhs (mk_u64 0)) 
           (Core_models.Abstractions.Bitvec.Int_vec_interp.e_ee_1__impl__to_i32x8 rhs (mk_u64 0))
-    ) = _ by (
+    ) = assert (
+        Core_models.Abstractions.Bitvec.Int_vec_interp.e_ee_1__impl__to_i32x8 (montgomery_multiply lhs rhs) (mk_u64 0)
+     == montgomery_multiply_spec 
+          (Core_models.Abstractions.Bitvec.Int_vec_interp.e_ee_1__impl__to_i32x8 lhs (mk_u64 0)) 
+          (Core_models.Abstractions.Bitvec.Int_vec_interp.e_ee_1__impl__to_i32x8 rhs (mk_u64 0))
+    ) by (
       let open FStar.Tactics in
       norm [iota; primops; delta_only [`%montgomery_multiply]; zeta];
       // l_to_r [`e_ee_1__lemma_cancel_iv'];
